tests/double_free.c
@@ -1,0 +1,9 @@
+#include "stdlib.h"
+
+int main() {
+	int* x = (int*) malloc(sizeof(int));
+	*x = 3;
+	free(x);
+	free(x);
+	return *x;
+}
