tests/heap_load_store_ib.c
@@ -1,0 +1,11 @@
+#include "stdlib.h"
+
+struct S {
+	int contents;
+};
+
+int main() {
+	struct S* s = (struct S*) malloc(sizeof(struct S));
+	s->contents = 42;
+	return s->contents;
+}
